%%%%%%%%%%%%%%%%%%%%%%%%%%%%%%%%%%%%%%%%%%%

\documentclass[11pt, a4paper, twoside]{article}
\usepackage[utf8]{inputenc}
\usepackage[T1]{fontenc}
\usepackage[francais]{babel}
\usepackage{lmodern}
\usepackage[margin=0.8in]{geometry}

\usepackage{amsmath}
\usepackage{amssymb}
\usepackage{amsthm}
\usepackage{mathrsfs}
\usepackage{mathtools}
\usepackage{enumitem}
\usepackage{graphicx}
\usepackage[all]{xy}

\DeclarePairedDelimiter\ceil{\lceil}{\rceil}
\DeclarePairedDelimiter\floor{\lfloor}{\rfloor}

\input{macrosMath}

%%%%%%%%%%%%%%%%%%%%%%%%%%%%%%%%%%%%%%%%%%%


\begin{document}
\title{Riemann Sufraces\\ Hand in 1}
\author{Christophe Marciot}
\maketitle

\section*{Exercise 1}
	Set $f(z)=\frac{az+b}{cz+d}$  where it is defined. Note that if $c=0$ then $d\neq0$ and $f(z)=\frac{a}{d}z+\frac{b}{d}$ is an affine map. If $c\neq0$ , one has $f=f_3\circ f_2\circ f_1$,where
		\begin{align*}
			f_1(z)&=cz+d,\\
			f_2(z)&=\frac{1}{z},\\
			f_3(z)&=\frac{bc-ad}{c}z+\frac{a}{c}.
		\end{align*}
	Now if we are able to show that afffine maps and $f_2$ send \emph{circles} to \emph{circles}. First let us investigate the case of affine maps. Let us set $g(z)=az+b,z=x+iy,a=\alpha+i\beta,b=\gamma+i\delta$. Note that we only care about the case where $a\neq0$. By computation, we obtain the following equation
		\begin{align*}
			u+iv=g(z)&=(\alpha+i\beta)(x+iy)+(\gamma+i\delta)\\
				        &=(\alpha x- \beta y +\gamma)+i(\beta x+\alpha y +\delta)
		\end{align*}
	which is equivalent to the system 
		$$\begin{cases}
			u=\alpha x-\beta y+\gamma,\\
			v=\beta x+\alpha y+\delta.
		\end{cases}$$
	We can inverse this system by the following computations 
		\begin{align*}
			\alpha u +\beta v=&\alpha^2x-\alpha\beta y+\alpha\gamma+\beta^2x+\alpha\beta y+\beta\delta\\
						      =&(\alpha^2+\beta^2)x+\alpha\gamma+\beta\delta\\
			&\iff\\
			x 				=& \frac{\alpha}{\alpha^2+\beta^2}(u-\gamma)+\frac{\beta}{\alpha^2+\beta^2}(v-\delta),\\
			\alpha v+\beta u =& (\alpha^2+\beta^2)y+\alpha\delta+\beta\gamma\\
			&\iff\\
			y				=& \frac{-\beta}{\alpha^2+\beta^2}(u-\gamma)+\frac{\alpha}{\alpha^2+\beta^2}(v-\delta)
		\end{align*}
	and we then get the system 
		$$\begin{cases}
			x = \frac{\alpha}{\alpha^2+\beta^2}(u-\gamma)+\frac{\beta}{\alpha^2+\beta^2}(v-\delta),\\
			y = \frac{-\beta}{\alpha^2+\beta^2}(u-\gamma)+\frac{\alpha}{\alpha^2+\beta^2}(v-\delta).
			\end{cases}$$
	Remember that we want to show that $g$ sends \emph{circles} to \emph{circles}. We treat the two cases separately:\\\\
	\underline{Case 1. $\lambda x+ \mu y = \nu$}, where $\lambda,\mu,\nu\in\RR$ and $\lambda$ or $\mu$ is nonzero (otherwise it would not be a line). We then get
		\begin{align*}
			\nu&= \lambda x+\mu y\\
				&=\lambda[\frac{\alpha}{\alpha^2+\beta^2}(u-\gamma)+\frac{\beta}{\alpha^2+\beta^2}(v-\delta)]+\mu[\frac{-\beta}{\alpha^2+\beta^2}(u-\gamma)+\frac{\alpha}{\alpha^2+\beta^2}(v-\delta)]\\
			     &= \frac{\lambda\alpha-\mu\beta}{\alpha^2+\beta^2}u+\frac{\mu\alpha+\lambda\beta}{\alpha^2+\beta^2}v-\frac{\lambda\alpha\gamma}{\alpha^2+\beta^2}-\frac{\lambda\beta\delta}{\alpha^2+\beta^2}+\frac{\mu\beta\gamma}{\alpha^2+\beta^2}-\frac{\mu\alpha\delta}{\alpha^2+\beta^2}\\
			     &= \frac{\lambda\alpha-\mu\beta}{\alpha^2+\beta^2}u+\frac{\mu\alpha+\lambda\beta}{\alpha^2+\beta^2}v-c\\
			\iff&\frac{\lambda\alpha-\mu\beta}{\alpha^2+\beta^2}u+\frac{\mu\alpha+\lambda\beta}{\alpha^2+\beta^2}v=\nu+c,
		\end{align*}
		where $c=\frac{\lambda\alpha\gamma+\lambda\beta\delta-\mu\beta\gamma+\mu\alpha\delta}{\alpha^2+\beta^2}$. Notice that this the equation of the line.\\\\
	\underline{Case 2. $(x-x_0)^2+(y-y_0)^2=R^2$}, where $x_0,y_0\in\RR$ and $R>0$. Note that the system of equations above gives us the following one 
		$$\begin{cases}
			x_0 = \frac{\alpha}{\alpha^2+\beta^2}(u_0-\gamma)+\frac{\beta}{\alpha^2+\beta^2}(v_0-\delta),\\
			y_0 = \frac{-\beta}{\alpha^2+\beta^2}(u_0-\gamma)+\frac{\alpha}{\alpha^2+\beta^2}(v_0-\delta).
			\end{cases}$$
		From this we can then compute what shape hase the image of this circle
		\begin{align*}
			R^2=& (x-x_0)^2+(y-y_0)^2\\
				=& [\frac{\alpha}{\alpha^2+\beta^2}(u-\gamma)+\frac{\beta}{\alpha^2+\beta^2}(v-\delta)-\frac{\alpha}{\alpha^2+\beta^2}(u_0-\gamma)-\frac{\beta}{\alpha^2+\beta^2}(v_0-\delta)]^2\\
				& + [\frac{-\beta}{\alpha^2+\beta^2}(u-\gamma)+\frac{\alpha}{\alpha^2+\beta^2}(v-\delta)-\frac{-\beta}{\alpha^2+\beta^2}(u_0-\gamma)-\frac{\alpha}{\alpha^2+\beta^2}(v_0-\delta)]^2\\
				=& [\frac{\alpha}{\alpha^2+\beta^2}(u-u_0)+\frac{\beta}{\alpha^2+\beta^2}(v-v_0)]^2+[\frac{-\beta}{\alpha^2+\beta^2}(u-u_0)+\frac{\alpha}{\alpha^2+\beta^2}(v-v_0)]^2
		\end{align*}
\end{document}
